EarleyTest/Basic.lean
@@ -155,36 +155,34 @@ instance : BEq G.NT where
 
 def exW1 : List (Symbol T N) := [Symbol.terminal T.a]
 def exW2 : List (Symbol T N) := [Symbol.terminal T.a, Symbol.terminal T.a, Symbol.terminal T.a]
-theorem finished1 : isFinished G exItem1 exW1 = false := rfl
-theorem finished2 : isFinished G exItem2 exW1 = false := rfl
-theorem finished3 : isFinished G exItem3 exW1 = false := rfl
-theorem finished4 : isFinished G exItem4 exW1 = false := rfl
-theorem finished5 : isFinished G exItem5 exW1 = true := rfl
+theorem finished1 : isFinished G exW1 exItem1 = false := rfl
+theorem finished2 : isFinished G exW1 exItem2 = false := rfl
+theorem finished3 : isFinished G exW1 exItem3 = false := rfl
+theorem finished4 : isFinished G exW1 exItem4 = false := rfl
+theorem finished5 : isFinished G exW1 exItem5 = true := rfl
 
 -- These just wait for lemmas, which I will require anyway for the proofs right?
   -- [Finset.mem_toList]
-theorem wf1 : isWellFormed G exItem1 exW1 := by
+theorem wf1 : isWellFormed G exW1 exItem1 := by
   rw [isWellFormed, exItem1]
   unfold G
   unfold exRules
   simp
-  sorry
 
-theorem wf2 : ¬isWellFormed G exItem2 exW1 := by
+theorem wf2 : ¬isWellFormed G exW1 exItem2 := by
   rw [isWellFormed, exItem2, exW1]
   simp [List.length]
 
-theorem wf3 : ¬isWellFormed G exItem3 exW2 := by
+theorem wf3 : ¬isWellFormed G exW2 exItem3 := by
   rw [isWellFormed, exItem3]
   simp
 
-theorem wf4 : ¬isWellFormed G exItem4 exW2 := by
+theorem wf4 : ¬isWellFormed G exW2 exItem4 := by
   rw [isWellFormed, exItem4, exItem1, exW2, exRule2]
   simp [List.length]
 
-theorem wf5 : isWellFormed G exItem5 exW2 := by
+theorem wf5 : isWellFormed G exW2 exItem5 := by
   rw [isWellFormed, exItem5, exW2]
   unfold G
   unfold exRules
-  simp [List.length]
-  sorry
+  simp [List.length, exRule1]
